STLC/PatternMatch.v
@@ -1,40 +1,58 @@
 From STLC Require Export Initial.
 
-Module pattern_match_version.
+(*CPS conversion rule*)
+(*
+  For an application [M1 M2], we can translate it into such a
+  manner:
+
+  if both are not recursive, we apply it to the continuation
+  function k :
+        [M1 M2] = k (M1 M2)
+
+  if only M1 is recursive, that's to say M1 admit another
+  parameter :
+        [M1 M2] = [M1] (fun hole => k (hole M2))
+
+  if only M2 is recursive, that's to say M2 admit another
+  parameter :
+        [M1 M2] = [M2] (fun hole => k (M1 hole))
+
+  if both are recursive :
+        [M1 M2] = [M1] (fun hole1 => [M2] (fun hole2 => k (hole1 hole2)))
+*)
 
 (*
   Deal with complicated pattern match, no longer using an extra parameter [fuel] to get accepted.
 *)
 
-Fixpoint CPS (continuation_name : string) (output_type: ty) (func_name : string) (func_body : tm) (naming : nat) (k : tm -> tm) {struct func_body} : tm :=
-  if is_recu func_name func_body then
-  let para_name := append "res" (nat2string naming) in
-  let result := k (var para_name) in
-  app func_body (abs para_name output_type
-  match find_func func_name result with
-       | O => app (var continuation_name) result
-       | S n1 => result
-       end)
-  else match func_body with
+Fixpoint CPS (continuation_name : string) (func_name : string) (func_body : tm) (naming : nat) (k : tm -> tm) {struct func_body} : tm :=
+  match func_body with
   | var _ =>
        let result := k func_body in
        match find_func func_name result with
        | O => app (var continuation_name) result
        | S n1 => result
        end
-  | abs x1 T t1 =>
-       abs x1 T (CPS continuation_name output_type func_name t1 naming k)
+  | abs x1 t1 =>
+       abs x1 (CPS continuation_name func_name t1 naming k)
   | app t1 t2 =>
-       match find_func func_name t1, find_func func_name t2 with
+       if is_recu func_name func_body then
+       let para_name := append "res" (nat2string naming) in
+       let result := k (var para_name) in
+       app func_body (abs para_name match find_func func_name result with
+                                                | O => app (var continuation_name) result
+                                                | S n1 => result
+                                                end)
+       else match find_func func_name t1, find_func func_name t2 with
        | O, O =>
             app (var continuation_name) (k func_body)
        | S n1, O =>
-            CPS continuation_name output_type func_name t1 naming (fun res : tm => k (app res t2))
+            CPS continuation_name func_name t1 naming (fun res : tm => k (app res t2))
        | O, S n2 =>
-            CPS continuation_name output_type func_name t2 naming (fun res : tm => k (app t1 res))
+            CPS continuation_name func_name t2 naming (fun res : tm => k (app t1 res))
        | S n1, S n2 =>
-            CPS continuation_name output_type func_name t1 naming
-            (fun res1 : tm => CPS continuation_name output_type func_name t2 (naming + (S n1))
+            CPS continuation_name func_name t1 naming
+            (fun res1 : tm => CPS continuation_name func_name t2 (naming + (S n1))
             (fun res2 : tm => k (app res1 res2)))
        end
   
@@ -49,12 +67,12 @@ Fixpoint CPS (continuation_name : string) (output_type: ty) (func_name : string)
        | O, O =>
             app (var continuation_name) (k func_body)
        | S n1, O =>
-            CPS continuation_name output_type func_name t1 naming (fun res : tm => k (tplus res t2))
+            CPS continuation_name func_name t1 naming (fun res : tm => k (tplus res t2))
        | O, S n2 =>
-            CPS continuation_name output_type func_name t2 naming (fun res : tm => k (tplus t1 res))
+            CPS continuation_name func_name t2 naming (fun res : tm => k (tplus t1 res))
        | S n1, S n2 =>
-            CPS continuation_name output_type func_name t1 naming
-            (fun res1 : tm => CPS continuation_name output_type func_name t2 (naming + (S n1))
+            CPS continuation_name func_name t1 naming
+            (fun res1 : tm => CPS continuation_name func_name t2 (naming + (S n1))
             (fun res2 : tm => k (tplus res1 res2)))
        end
   | tminus t1 t2 =>
@@ -62,12 +80,12 @@ Fixpoint CPS (continuation_name : string) (output_type: ty) (func_name : string)
        | O, O =>
             app (var continuation_name) (k func_body)
        | S n1, O =>
-            CPS continuation_name output_type func_name t1 naming (fun res : tm => k (tminus res t2))
+            CPS continuation_name func_name t1 naming (fun res : tm => k (tminus res t2))
        | O, S n2 =>
-            CPS continuation_name output_type func_name t2 naming (fun res : tm => k (tminus t1 res))
+            CPS continuation_name func_name t2 naming (fun res : tm => k (tminus t1 res))
        | S n1, S n2 =>
-            CPS continuation_name output_type func_name t1 naming
-            (fun res1 : tm => CPS continuation_name output_type func_name t2 (naming + (S n1))
+            CPS continuation_name func_name t1 naming
+            (fun res1 : tm => CPS continuation_name func_name t2 (naming + (S n1))
             (fun res2 : tm => k (tminus res1 res2)))
        end
   | tmult t1 t2 =>
@@ -75,21 +93,21 @@ Fixpoint CPS (continuation_name : string) (output_type: ty) (func_name : string)
        | O, O =>
             app (var continuation_name) (k func_body)
        | S n1, O =>
-            CPS continuation_name output_type func_name t1 naming (fun res : tm => k (tmult res t2))
+            CPS continuation_name func_name t1 naming (fun res : tm => k (tmult res t2))
        | O, S n2 =>
-            CPS continuation_name output_type func_name t2 naming (fun res : tm => k (tmult t1 res))
+            CPS continuation_name func_name t2 naming (fun res : tm => k (tmult t1 res))
        | S n1, S n2 =>
-            CPS continuation_name output_type func_name t1 naming
-            (fun res1 : tm => CPS continuation_name output_type func_name t2 (naming + (S n1))
+            CPS continuation_name func_name t1 naming
+            (fun res1 : tm => CPS continuation_name func_name t2 (naming + (S n1))
             (fun res2 : tm => k (tmult res1 res2)))
        end
   | tif0 t1 t2 t3 =>
        match find_func func_name t1 with
-       | O => tif0 t1 (CPS continuation_name output_type func_name t2 naming k) (CPS continuation_name output_type func_name t3 naming k)
-       | S n1 => CPS continuation_name output_type func_name t1 naming (fun res : tm => k (tif0 res t2 t3))
+       | O => tif0 t1 (CPS continuation_name func_name t2 naming k) (CPS continuation_name func_name t3 naming k)
+       | S n1 => CPS continuation_name func_name t1 naming (fun res : tm => k (tif0 res t2 t3))
        end
   
-  | tnil _ =>
+  | tnil =>
        let result := k func_body in
        match find_func func_name result with
        | O => app (var continuation_name) result
@@ -100,75 +118,33 @@ Fixpoint CPS (continuation_name : string) (output_type: ty) (func_name : string)
        | O, O =>
             app (var continuation_name) (k func_body)
        | S n1, O =>
-            CPS continuation_name output_type func_name t1 naming (fun res : tm => k (tcons res t2))
+            CPS continuation_name func_name t1 naming (fun res : tm => k (tcons res t2))
        | O, S n2 =>
-            CPS continuation_name output_type func_name t2 naming (fun res : tm => k (tcons t1 res))
+            CPS continuation_name func_name t2 naming (fun res : tm => k (tcons t1 res))
        | S n1, S n2 =>
-            CPS continuation_name output_type func_name t1 naming
-            (fun res1 : tm => CPS continuation_name output_type func_name t2 (naming + (S n1))
+            CPS continuation_name func_name t1 naming
+            (fun res1 : tm => CPS continuation_name func_name t2 (naming + (S n1))
             (fun res2 : tm => k (tcons res1 res2)))
        end
   | tlcase t1 t2 x1 x2 t3 =>
        match find_func func_name t1 with
-       | O => tlcase t1 (CPS continuation_name output_type func_name t2 naming k) x1 x2 (CPS continuation_name output_type func_name t3 naming k)
-       | S n1 => CPS continuation_name output_type func_name t1 naming (fun res : tm => k (tlcase res t2 x1 x2 t3))
-       end
-  
-  | tleaf t1 =>
-       match find_func func_name t1 with
-       | O => app (var continuation_name) (k func_body)
-       | S n1 => CPS continuation_name output_type func_name t1 naming (fun res : tm => k (tleaf res))
-       end
-  | tnode t1 t2 t3 =>
-       match find_func func_name t1, find_func func_name t2, find_func func_name t3 with
-       | O, O, O =>
-            app (var continuation_name) (k func_body)
-       | S n1, O, O =>
-            CPS continuation_name output_type func_name t1 naming (fun res : tm => k (tnode res t2 t3))
-       | O, S n2, O =>
-            CPS continuation_name output_type func_name t2 naming (fun res : tm => k (tnode t1 res t3))
-       | O, O, S n3 =>
-            CPS continuation_name output_type func_name t3 naming (fun res : tm => k (tnode t1 t2 res))
-       | S n1, S n2, O =>
-            CPS continuation_name output_type func_name t1 naming
-            (fun res1 : tm => CPS continuation_name output_type func_name t2 (naming + (S n1))
-            (fun res2 : tm => k (tnode res1 res2 t3)))
-       | S n1, O, S n3 =>
-            CPS continuation_name output_type func_name t1 naming
-            (fun res1 : tm => CPS continuation_name output_type func_name t3 (naming + (S n1))
-            (fun res2 : tm => k (tnode res1 t2 res2)))
-       | O, S n2, S n3 =>
-            CPS continuation_name output_type func_name t2 naming
-            (fun res1 : tm => CPS continuation_name output_type func_name t3 (naming + (S n2))
-            (fun res2 : tm => k (tnode t1 res1 res2)))
-       | S n1, S n2, S n3 =>
-            CPS continuation_name output_type func_name t1 naming
-            (fun res1 : tm => CPS continuation_name output_type func_name t2 (naming + (S n1))
-            (fun res2 : tm => CPS continuation_name output_type func_name t3 (naming + (S n1)+ (S n2))
-            (fun res3 : tm => k (tnode res1 res2 res3))))
-       end
-  | tbcase t1 x1 t2 x2 x3 x4 t3 =>
-       match find_func func_name t1 with
-       | O => tbcase t1 x1 (CPS continuation_name output_type func_name t2 naming k) x2 x3 x4 (CPS continuation_name output_type func_name t3 naming k)
-       | S n1 => CPS continuation_name output_type func_name t1 naming (fun res : tm => k (tbcase res x1 t2 x2 x3 x4 t3))
+       | O => tlcase t1 (CPS continuation_name func_name t2 naming k) x1 x2 (CPS continuation_name func_name t3 naming k)
+       | S n1 => CPS continuation_name func_name t1 naming (fun res : tm => k (tlcase res t2 x1 x2 t3))
        end
   
   | tlet x1 t1 t2 =>
-       tlet x1 (CPS continuation_name output_type func_name t1 naming k) (CPS continuation_name output_type func_name t2 naming k)
+       tlet x1 (CPS continuation_name func_name t1 naming k) (CPS continuation_name func_name t2 naming k)
   
   | tfix t1 =>
-       tfix (CPS continuation_name output_type func_name t1 naming k)
+       tfix (CPS continuation_name func_name t1 naming k)
   end.
 
 Definition CPS_conversion (func : tm) : tm :=
   match func with
-  | tfix (abs func_name func_type func_body) =>
-       let output_type := get_output_type func_type in
+  | tfix (abs func_name func_body) =>
        let continuation_name := k in
-       let continuation_type := Arrow output_type output_type in
-       let func_new_type := type_insert func_type continuation_type in
-       let func_paraed_body := para_insert continuation_name continuation_type func_body in
-       tfix (abs func_name func_new_type (CPS continuation_name output_type func_name func_paraed_body 1 (fun res : tm => res)))
+       let func_paraed_body := para_insert continuation_name func_body in
+       tfix (abs func_name (CPS continuation_name func_name func_paraed_body 1 (fun res : tm => res)))
   | _ => func
   end.
 
@@ -177,8 +153,8 @@ Definition CPS_conversion (func : tm) : tm :=
 Module examples.
 
 Definition stlc_match_case1 :=
-  tfix (abs F (Arrow (List Nat) Nat)
-    (abs l (List Nat)
+  tfix (abs F
+    (abs l
       (tlcase l 0 n1 l1
         (tlcase l1 n1 n2 l2
           (tplus n1 (tplus n2 (app F l2))))))).
@@ -188,14 +164,14 @@ Compute (CPS_conversion stlc_match_case1).
 Theorem stlc_match_case1_correct :
   let origin_fun := stlc_match_case1 in
   let CPS_fun := CPS_conversion stlc_match_case1 in
-  let input := tcons 4 (tcons 3 (tcons 1 (tcons 2 (tnil Nat)))) in
+  let input := tcons 4 (tcons 3 (tcons 1 (tcons 2 tnil))) in
   let output := 10 in
   (<{origin_fun input}> -->* output) /\ (<{CPS_fun input idNat}> -->* output).
 Proof. split. solve_CPS. solve_CPS. Qed.
 
 Definition stlc_match_case2 :=
-  tfix (abs F (Arrow (List Nat) Nat)
-    (abs l (List Nat)
+  tfix (abs F
+    (abs l
       (tplus 1 (tlcase l 0 n1 l1
         (tplus n1 (app F l1)))))).
 
@@ -204,14 +180,14 @@ Compute (CPS_conversion stlc_match_case2).
 Theorem stlc_match_case2_correct :
   let origin_fun := stlc_match_case2 in
   let CPS_fun := CPS_conversion stlc_match_case2 in
-  let input := tcons 4 (tcons 3 (tcons 1 (tcons 2 (tnil Nat)))) in
+  let input := tcons 4 (tcons 3 (tcons 1 (tcons 2 tnil))) in
   let output := 15 in
   (<{origin_fun input}> -->* output) /\ (<{CPS_fun input idNat}> -->* output).
 Proof. split. solve_CPS. solve_CPS. Qed.
 
 Definition stlc_match_case3 :=
-  tfix (abs F (Arrow (List Nat) Nat)
-    (abs l (List Nat)
+  tfix (abs F
+    (abs l
       (tlcase l 0 n1 l1
         (tif0 (app F l1) n1 (tmult 2 n1))))).
 
@@ -220,15 +196,15 @@ Compute (CPS_conversion stlc_match_case3).
 Theorem stlc_match_case3_correct :
   let origin_fun := stlc_match_case3 in
   let CPS_fun := CPS_conversion stlc_match_case3 in
-  let input := tcons 2 (tcons 2 (tnil Nat)) in
+  let input := tcons 2 (tcons 2 tnil) in
   let output := 4 in
   (<{origin_fun input}> -->* output) /\ (<{CPS_fun input idNat}> -->* output).
 Proof. split. solve_CPS. solve_CPS. Qed.
 
 Definition stlc_match_case4 :=
-  tfix (abs F (Arrow (List Nat) (Arrow (List Nat) Nat))
-    (abs l1 (List Nat)
-       (abs l2 (List Nat)
+  tfix (abs F
+    (abs l1
+       (abs l2
          (tplus (tlcase l1 0 n1 l'
            (tplus n1 (app (app F l') l2)))
              (tlcase l2 0 n2 l''
@@ -239,15 +215,15 @@ Compute (CPS_conversion stlc_match_case4).
 Theorem stlc_match_case4_correct :
   let origin_fun := stlc_match_case4 in
   let CPS_fun := CPS_conversion stlc_match_case4 in
-  let input1 := tcons 2 (tcons 3 (tcons 5 (tnil Nat))) in
-  let input2 := tcons 4 (tcons 2 (tnil Nat)) in
+  let input1 := tcons 2 (tcons 3 (tcons 5 tnil)) in
+  let input2 := tcons 4 (tcons 2 tnil) in
   let output := 110 in
   (<{origin_fun input1 input2}> -->* output) /\ (<{CPS_fun input1 input2 idNat}> -->* output).
 Proof. split. solve_CPS. solve_CPS. Qed.
 
 Definition stlc_match_case5 :=
-  tfix (abs F (Arrow (List Nat) Nat)
-    (abs l (List Nat)
+  tfix (abs F
+    (abs l
       (tplus 3 (tmult (tlcase l (tminus 2 1) n1 l'
         (tplus n1 (tplus 1 (tplus (app F l') 1)))) 5)))).
 
@@ -256,11 +232,9 @@ Compute (CPS_conversion stlc_match_case5).
 Theorem stlc_match_case5_correct :
   let origin_fun := stlc_match_case5 in
   let CPS_fun := CPS_conversion stlc_match_case5 in
-  let input := tcons 2 (tcons 3 (tcons 5 (tnil Nat))) in
+  let input := tcons 2 (tcons 3 (tcons 5 tnil)) in
   let output := 2113 in
   (<{origin_fun input}> -->* output) /\ (<{CPS_fun input idNat}> -->* output).
 Proof. split. solve_CPS. solve_CPS. Qed.
 
 End examples.
-
-End pattern_match_version.
