STLC/Proof.v
@@ -1,0 +1,449 @@
+From STLC Require Export Definitions.
+From STLC Require Export Argument.
+From Coq Require Import Logic.FunctionalExtensionality.
+(*From Coq Require Import List.
+Import ListNotations.*)
+
+Print tm.
+Print depth.
+Print CPS.
+
+Inductive stlc_expr (func_name : string) : tm -> Prop :=
+  | E_Var : forall x1,
+        eqb func_name x1 = false ->
+        stlc_expr func_name (var x1)
+  | E_Abs : forall x1 t1 t2,
+       eqb func_name x1 = false ->
+       stlc_expr func_name t1 ->
+       stlc_expr func_name t2 ->
+       stlc_expr func_name (app (abs x1 t1) t2)
+  | E_AppF : forall t1,
+       stlc_expr func_name t1 ->
+       stlc_expr func_name (app (var func_name) t1)
+  | E_App : forall t1 t2,
+       stlc_expr func_name t1 ->
+       stlc_expr func_name t2 ->
+       stlc_expr func_name (app t1 t2)
+  
+  | E_Const : forall n,
+       stlc_expr func_name (tconst n)
+  | E_Plus : forall t1 t2,
+       stlc_expr func_name t1 ->
+       stlc_expr func_name t2 ->
+       stlc_expr func_name (tplus t1 t2)
+  | E_Minus : forall t1 t2,
+       stlc_expr func_name t1 ->
+       stlc_expr func_name t2 ->
+       stlc_expr func_name (tminus t1 t2)
+  | E_Mult : forall t1 t2,
+       stlc_expr func_name t1 ->
+       stlc_expr func_name t2 ->
+       stlc_expr func_name (tmult t1 t2)
+  | E_If0 : forall t1 t2 t3,
+       stlc_expr func_name t1 ->
+       stlc_expr func_name t2 ->
+       stlc_expr func_name t3 ->
+       stlc_expr func_name (tif0 t1 t2 t3)
+  
+  | E_Nil :
+       stlc_expr func_name tnil
+  | E_Cons : forall t1 t2,
+       stlc_expr func_name t1 ->
+       stlc_expr func_name t2 ->
+       stlc_expr func_name (tcons t1 t2)
+  | E_LCase : forall t1 t2 x1 x2 t3,
+       eqb func_name x1 = false ->
+       eqb func_name x2 = false ->
+       stlc_expr func_name t1 ->
+       stlc_expr func_name t2 ->
+       stlc_expr func_name t3 ->
+       stlc_expr func_name (tlcase t1 t2 x1 x2 t3)
+
+  | E_Let : forall x1 t1 t2,
+       eqb func_name x1 = false ->
+       stlc_expr func_name t1 ->
+       stlc_expr func_name t2 ->
+       stlc_expr func_name (tlet x1 t1 t2).
+
+Reserved Notation "t1 '=s' t2" (at level 50).
+
+Inductive stlc_eqb : tm -> tm -> Prop :=
+  | S_Refl : forall x1,
+       x1 =s x1
+  | S_Symm : forall x1 x2,
+       x1 =s x2 ->
+       x2 =s x1
+  | S_Trans : forall x1 x2 x3,
+       x1 =s x2 ->
+       x2 =s x3 ->
+       x1 =s x3
+  
+  | S_App : forall t1 t1' t2 t2',
+       t1 =s t1' ->
+       t2 =s t2' ->
+       app t1 t2 =s app t1' t2'
+  | S_AppAbs : forall x y t,
+       app (abs x t) y =s subst x y t
+  | S_Abs : forall x t t',
+       t =s t' ->
+       abs x t =s abs x t'
+  | S_AbsName : forall x y t,
+       (List.In y (list_name t) -> False) ->
+       abs x t =s abs y (subst x y t)
+  
+  | S_Plus : forall t1 t1' t2 t2',
+       t1 =s t1' ->
+       t2 =s t2' ->
+       tplus t1 t2 =s tplus t1' t2'
+  | S_Minus : forall t1 t1' t2 t2',
+       t1 =s t1' ->
+       t2 =s t2' ->
+       tminus t1 t2 =s tminus t1' t2'
+  | S_Mult : forall t1 t1' t2 t2',
+       t1 =s t1' ->
+       t2 =s t2' ->
+       tmult t1 t2 =s tmult t1' t2'
+  | S_If0 : forall t1 t1' t2 t2' t3 t3',
+       t1 =s t1' ->
+       t2 =s t2' ->
+       t3 =s t3' ->
+       tif0 t1 t2 t3 =s tif0 t1' t2' t3'
+  | S_If0AppLeft : forall k t1 t2 t3,
+       app k (tif0 t1 t2 t3) =s tif0 t1 (app k t2) (app k t3)
+  | S_If0AppRight : forall k t1 t2 t3,
+       app (tif0 t1 t2 t3) k =s tif0 t1 (app t2 k) (app t3 k)
+  
+  | S_Cons : forall t1 t1' t2 t2',
+       t1 =s t1' ->
+       t2 =s t2' ->
+       tcons t1 t2 =s tcons t1' t2'
+  | S_LCase : forall t1 t1' t2 t2' x1 x2 t3 t3',
+       t1 =s t1' ->
+       t2 =s t2' ->
+       t3 =s t3' ->
+       tlcase t1 t2 x1 x2 t3 =s tlcase t1' t2' x1 x2 t3'
+  | S_LCaseAppLeft : forall k t1 t2 x1 x2 t3,
+       app k (tlcase t1 t2 x1 x2 t3) =s tlcase t1 (app k t2) x1 x2 (app k t3)
+  | S_LCaseAppRight : forall k t1 t2 x1 x2 t3,
+       app (tlcase t1 t2 x1 x2 t3) k =s tlcase t1 (app t2 k) x1 x2 (app t3 k)
+  
+  | S_Let : forall x t1 t1' t2 t2',
+       t1 =s t1' ->
+       t2 =s t2' ->
+       tlet x t1 t2 =s tlet x t1' t2'
+  | S_LetSubst : forall x t1 t2,
+       tlet x t1 t2 =s subst x t1 t2
+  
+  | S_Fix : forall t1 t1',
+       t1 =s t1' ->
+       tfix t1 =s tfix t1'
+  | S_FixAbs : forall f t,
+       tfix (abs f t) =s subst f (tfix (abs f t)) t
+
+  where "t1 '=s' t2" := (stlc_eqb t1 t2).
+
+Lemma depth_helper1 :
+  forall m, exists n, S m = S n.
+Proof.
+  intros m. exists m. reflexivity.
+Qed.
+
+Lemma depth_gt_1 :
+  forall F M, exists n, depth F M = S n.
+Proof.
+  intros. destruct M; simpl; try (apply depth_helper1); try (destruct (find_func F M1), (find_func F M2); apply depth_helper1).
+  - destruct ((find_func F M1 =? 1) && (find_func F M2 =? 0) && is_recu F M1)%bool. apply depth_helper1.
+  destruct (find_func F M1), (find_func F M2); apply depth_helper1.
+Qed.
+
+Lemma depth_helper2 :
+  forall n m, exists k, n + k = Init.Nat.max n m.
+Proof.
+  Search "<=". intros. induction (Nat.le_max_l n m).
+  - exists 0. apply Nat.add_comm.
+  - destruct IHl. exists (S x). rewrite Nat.add_comm. simpl. f_equal. rewrite Nat.add_comm. apply H.
+Qed.
+
+Axiom stlc_functional_extensionality : forall (A : Type) (f g : A -> tm),
+  (forall x : A, f x =s g x) -> f = g.
+
+Theorem fuel_enough :
+  forall k F M continuation naming n,
+  CPS k F M continuation naming (depth F M) =s CPS k F M continuation naming (depth F M + n).
+Proof.
+  intros. generalize dependent naming. generalize dependent continuation. generalize dependent n. induction M.
+  - intros n H naming. destruct (depth_gt_1 F <{ s }>). rewrite H0. simpl. apply S_Refl.
+  - admit.
+  - intros n H naming. destruct (depth_gt_1 F <{ \ s, M }>). simpl in H0. injection H0 as H0. simpl. apply S_Abs. apply IHM.
+  - intros. simpl. apply S_Refl.
+  - intros n H naming. destruct (depth_gt_1 F <{ M1 + M2 }>). rewrite H0. simpl in H0. simpl. destruct (find_func F M1), (find_func F M2); injection H0 as H0; try (rewrite <- H0).
+    apply S_Refl. apply IHM2. apply IHM1. destruct (depth_helper2 (depth F M1) (depth F M2)). rewrite <- H1. eapply S_Trans. apply S_Symm. apply IHM1. rewrite Plus.plus_assoc_reverse.
+    assert ((fun res1 : tm => CPS k F M2 (fun res2 : tm => H <{ res1 + res2 }>) (naming + S n0) (depth F M1 + x0)) = (fun res1 : tm => CPS k F M2 (fun res2 : tm => H <{ res1 + res2 }>) (naming + S n0) (depth F M1 + (x0 + n)))). {
+    apply stlc_functional_extensionality. intros. rewrite <- Plus.plus_assoc_reverse. rewrite H1. destruct (depth_helper2 (depth F M2) (depth F M1)). rewrite Nat.max_comm in H2. rewrite <- H2. eapply S_Trans. apply S_Symm.
+    apply (IHM2 x2 (fun res2 : tm => H <{ x1 + res2 }>) (naming + S n0)). rewrite Plus.plus_assoc_reverse. apply IHM2. } rewrite H2. apply IHM1.
+  - intros n H naming. destruct (depth_gt_1 F <{ M1 - M2 }>). rewrite H0. simpl in H0. simpl. destruct (find_func F M1), (find_func F M2); injection H0 as H0; try (rewrite <- H0).
+    apply S_Refl. apply IHM2. apply IHM1. destruct (depth_helper2 (depth F M1) (depth F M2)). rewrite <- H1. eapply S_Trans. apply S_Symm. apply IHM1. rewrite Plus.plus_assoc_reverse.
+    assert ((fun res1 : tm => CPS k F M2 (fun res2 : tm => H <{ res1 - res2 }>) (naming + S n0) (depth F M1 + x0)) = (fun res1 : tm => CPS k F M2 (fun res2 : tm => H <{ res1 - res2 }>) (naming + S n0) (depth F M1 + (x0 + n)))). {
+    apply stlc_functional_extensionality. intros. rewrite <- Plus.plus_assoc_reverse. rewrite H1. destruct (depth_helper2 (depth F M2) (depth F M1)). rewrite Nat.max_comm in H2. rewrite <- H2. eapply S_Trans. apply S_Symm.
+    apply (IHM2 x2 (fun res2 : tm => H <{ x1 - res2 }>) (naming + S n0)). rewrite Plus.plus_assoc_reverse. apply IHM2. } rewrite H2. apply IHM1.
+  - intros n H naming. destruct (depth_gt_1 F <{ M1 * M2 }>). rewrite H0. simpl in H0. simpl. destruct (find_func F M1), (find_func F M2); injection H0 as H0; try (rewrite <- H0).
+    apply S_Refl. apply IHM2. apply IHM1. destruct (depth_helper2 (depth F M1) (depth F M2)). rewrite <- H1. eapply S_Trans. apply S_Symm. apply IHM1. rewrite Plus.plus_assoc_reverse.
+    assert ((fun res1 : tm => CPS k F M2 (fun res2 : tm => H <{ res1 * res2 }>) (naming + S n0) (depth F M1 + x0)) = (fun res1 : tm => CPS k F M2 (fun res2 : tm => H <{ res1 * res2 }>) (naming + S n0) (depth F M1 + (x0 + n)))). {
+    apply stlc_functional_extensionality. intros. rewrite <- Plus.plus_assoc_reverse. rewrite H1. destruct (depth_helper2 (depth F M2) (depth F M1)). rewrite Nat.max_comm in H2. rewrite <- H2. eapply S_Trans. apply S_Symm.
+    apply (IHM2 x2 (fun res2 : tm => H <{ x1 * res2 }>) (naming + S n0)). rewrite Plus.plus_assoc_reverse. apply IHM2. } rewrite H2. apply IHM1.
+  - intros n H naming. destruct (depth_gt_1 F <{ if0 M1 then M2 else M3 }>). rewrite H0. simpl in H0. simpl. destruct (find_func F M1). injection H0 as H0. apply S_If0. apply S_Refl. rewrite <- H0.
+    destruct (depth_helper2 (depth F M2) (depth F M3)). rewrite <- H1. eapply S_Trans. apply S_Symm. apply IHM2. rewrite Plus.plus_assoc_reverse. apply IHM2. destruct (depth_helper2 (depth F M3) (depth F M2)). rewrite Nat.max_comm in H1.
+    rewrite <- H0. rewrite <- H1. eapply S_Trans. apply S_Symm. apply IHM3. rewrite Plus.plus_assoc_reverse. apply IHM3. injection H0 as H0. rewrite <- H0. apply IHM1.
+  - intros n H naming. simpl. apply S_Refl.
+  - intros n H naming. destruct (depth_gt_1 F <{ M1 :: M2 }>). rewrite H0. simpl in H0. simpl. destruct (find_func F M1), (find_func F M2); injection H0 as H0; try (rewrite <- H0).
+    apply S_Refl. apply IHM2. apply IHM1. destruct (depth_helper2 (depth F M1) (depth F M2)). rewrite <- H1. eapply S_Trans. apply S_Symm. apply IHM1. rewrite Plus.plus_assoc_reverse.
+    assert ((fun res1 : tm => CPS k F M2 (fun res2 : tm => H <{ res1 :: res2 }>) (naming + S n0) (depth F M1 + x0)) = (fun res1 : tm => CPS k F M2 (fun res2 : tm => H <{ res1 :: res2 }>) (naming + S n0) (depth F M1 + (x0 + n)))). {
+    apply stlc_functional_extensionality. intros. rewrite <- Plus.plus_assoc_reverse. rewrite H1. destruct (depth_helper2 (depth F M2) (depth F M1)). rewrite Nat.max_comm in H2. rewrite <- H2. eapply S_Trans. apply S_Symm.
+    apply (IHM2 x2 (fun res2 : tm => H <{ x1 :: res2 }>) (naming + S n0)). rewrite Plus.plus_assoc_reverse. apply IHM2. } rewrite H2. apply IHM1.
+  - intros n H naming. destruct (depth_gt_1 F <{ case M1 of | nil => M2 | s :: s0 => M3 }>). rewrite H0. simpl in H0. simpl. destruct (find_func F M1). injection H0 as H0. apply S_LCase. apply S_Refl. rewrite <- H0.
+    destruct (depth_helper2 (depth F M2) (depth F M3)). rewrite <- H1. eapply S_Trans. apply S_Symm. apply IHM2. rewrite Plus.plus_assoc_reverse. apply IHM2. destruct (depth_helper2 (depth F M3) (depth F M2)). rewrite Nat.max_comm in H1.
+    rewrite <- H0. rewrite <- H1. eapply S_Trans. apply S_Symm. apply IHM3. rewrite Plus.plus_assoc_reverse. apply IHM3. injection H0 as H0. rewrite <- H0. apply IHM1.
+  - intros n H naming. simpl. apply S_Let. destruct (depth_helper2 (depth F M1) (depth F M2)). rewrite <- H0. eapply S_Trans. apply S_Symm. apply IHM1. rewrite Plus.plus_assoc_reverse. apply IHM1.
+    destruct (depth_helper2 (depth F M2) (depth F M1)). rewrite Nat.max_comm in H0. rewrite <- H0. eapply S_Trans. apply S_Symm. apply IHM2. rewrite Plus.plus_assoc_reverse. apply IHM2.
+  - intros n H naming. simpl. apply S_Fix. apply IHM.
+  Admitted.
+
+Theorem naming_arbitrarility :
+  forall k F M continuation n,
+  CPS k F M continuation 1 (depth F M) =s CPS k F M continuation (1 + n) (depth F M).
+
+Theorem CPS_conversion_correct : forall F f f' k M,
+  subst F f k =s k ->
+  subst F f' k =s k ->
+  stlc_expr F M ->
+  subst F f' (CPS k F M (fun res => res) 1 (depth F M)) =s app k (subst F f M).
+Proof.
+  intros. rename H into Hkf. rename H0 into Hkf'. rename H1 into H. remember M as HM. induction M; rewrite HeqHM in *; simpl.
+  - inversion H. rewrite (eqb_sym s F). rewrite H1. simpl. rewrite H1. apply S_App. apply Hkf'. apply S_Refl.
+  - admit.
+  - inversion H.
+  - apply S_App. apply Hkf'. apply S_Refl.
+  - Admitted.
+
+(*
+  The definition of [stlc_eqb] :
+
+                    -----------------------------                       (S_Refl)
+                               x1 =s x1
+
+                               x1 =s x2
+                    -----------------------------                       (S_Symm)
+                               x2 =s x1
+
+                               x1 =s x2
+                               x2 =s x3
+                    -----------------------------                       (S_Trans)
+                               x1 =s x3
+
+                              t1 =s t1'
+                              t2 =s t2'
+                    -------------------------------                     (S_App)
+                        app t1 t2 =s app t1' t2'
+
+                    --------------------------------                    (S_AppAbs)
+                     app (abs x t) y =s subst x y t
+
+                               t =s t'
+                    --------------------------------                    (S_Abs)
+                          abs x t =s abs x t'
+
+                        In y (list_name t) = false
+                    --------------------------------                    (S_AbsName)
+                          abs x t =s abs x t'
+
+                              t1 =s t1'
+                              t2 =s t2'
+                    ---------------------------------                   (S_Plus)
+                      tplus t1 t2 =s tplus t1' t2'
+
+                              t1 =s t1'
+                              t2 =s t2'
+                    ---------------------------------                   (S_Minus)
+                      tminus t1 t2 =s tminus t1' t2'
+
+                              t1 =s t1'
+                              t2 =s t2'
+                    ---------------------------------                   (S_Mult)
+                      tmult t1 t2 =s tmult t1' t2'
+
+                              t1 =s t1'
+                              t2 =s t2'
+                              t3 =s t3'
+                    ---------------------------------                   (S_If0)
+                      tif0 t1 t2 t3 =s t1' t2' t3'
+
+            -----------------------------------------------------       (S_If0AppLeft)
+            app k (tif0 t1 t2 t3) =s tif0 t1 (app k t2) (app k t3)
+
+            -----------------------------------------------------       (S_If0AppRight)
+            app (tif0 t1 t2 t3) k =s tif0 t1 (app t2 k) (app t3 k)
+
+                              t1 =s t1'
+                              t2 =s t2'
+                    ---------------------------------                   (S_Cons)
+                      tcons t1 t2 =s tcons t1' t2'
+
+                              t1 =s t1'
+                              t2 =s t2'
+                              t3 =s t3'
+                    ---------------------------------                   (S_LCase)
+                      tlcase t1 t2 x1 x2 t3 =s tlcase t1' t2' x1 x2 t3'
+
+            -----------------------------------------------------       (S_LCaseAppLeft)
+      app k (tlcase t1 t2 x1 x2 t3) =s tlcase t1 (app k t2) x1 x2 (app k t3)
+
+            -----------------------------------------------------       (S_LCaseAppRight)
+      app (tlcase t1 t2 x1 x2 t3) k =s tlcase t1 (app t2 k) x1 x2 (app t3 k)
+
+                              t1 =s t1'
+                    ---------------------------------                   (S_Fix)
+                         tfix t1 =s tfix t1'
+
+                    ---------------------------------                   (S_FixAbs)
+                 tfix (abs f t) =s subst f (tfix (abs f t)) t
+
+  The meanings of symbols:
+    F is the identifier of the recursive function.
+    f is the syntax tree before the CPS conversion.
+    f' is the syntax tree after the CPS conversion.
+    M is the recursive stlc expression consist in f, that is to say M is the remain part of f after removing those outer [abs]s.
+    k is the continuation.
+    Here, we suppose that there is no duplication of variable name.
+
+  A property of f and f':
+    forall k, app k (app f ...) = app (app f' ...) k,
+    where ... are the parameters of f.
+
+  Properties of M:
+    1. M is not of the form [abs _ _],
+    2. M does not contain [tfix],
+    3. Those variables bound in M do not contain F (resursive function name).
+
+  Properties of k:
+    k does not contain recursive call because we do not consider free variables.
+    Consequently we can get two lemmas:
+    1. subst F f k =s k
+    2. subst F f' k =s k
+
+  Our conversion function:
+    CPS (k : tm) (func_name : string) (func_body : tm) (continuation : tm -> tm) (naming fuel : nat),
+    where the initial values of [continuation], [naming] and [fuel] are respectively [fun res => res] 1 and [depth M].
+
+  The theorem to be informally proved:
+    subst F f' (CPS k F M (fun res => res) 1 (depth F M)) =s app k (subst F f M)
+
+  Proof:
+
+  By induction on M.
+
+  1. When M = var x1.
+     F is not equal to x1,
+          subst F f (var x1) = var x1
+          subst F f' (var x1) = var x1
+     We know that,
+          CPS k F (var x1) (fun res => res) 1 (depth F (var x1))
+       =s CPS k F (var x1) (fun res => res) 1 1
+       =s app k (var x1)
+     Finally,
+          subst F f' (CPS k F (var x1) (fun res => res) 1 (depth F (var x1)))
+       =s subst F f' (app k (var x1))
+       =s app (subst F f' k) (subst F f' (var x1))
+       =s app k (var x1)
+       =s app k (subst F f (var x1))
+
+  2. When M = app t1 t2.
+  
+  3. When M = tconst n.
+     We know that,
+          CPS k F (tconst n) (fun res => res) 1 (depth F (tconst n))
+       =s CPS k F (tconst n) (fun res => res) 1 1
+       =s app k (tconst n)
+     Finally,
+          subst F f' (CPS k F (tconst n) (fun res => res) 1 (depth F (tconst n)))
+       =s subst F f' (app k (tconst n))
+       =s app (subst F f' k) (subst F f' (tconst n))
+       =s app k (tconst n)
+       =s app k (subst F f (tconst n))
+
+  4. When M = tplus t1 t2.
+     The induction hypothesis:
+          subst F f' (CPS k F t1 (fun res => res) 1 (depth F t1)) =s app k (subst F f t1)
+          subst F f' (CPS k F t2 (fun res => res) 1 (depth F t2)) =s app k (subst F f t2)
+       ▲ If both t1 and t2 are not resursive,
+       We know that,
+            CPS k F (tplus t1 t2) (fun res => res) 1 (depth F (tplus t1 t2))
+         =s CPS k F (tplus t1 t2) (fun res => res) 1 1
+         =s app k (tplus t1 t2)
+       Finally,
+            subst F f' (CPS k F (tplus t1 t2) (fun res => res) 1 (depth F (tplus t1 t2)))
+         =s subst F f' (app k (tplus t1 t2))
+         =s app (subst F f' k) (tplus (subst F f' t1) (subst F f' t2))
+         =s app k (tplus t1 t2)
+         =s app k (tplus (subst F f t1) (subst F f t2))
+         =s app k (subst F f (tplus t1 t2))
+       ▲ If t1 is recursive and t2 not recursive,
+       We know that,
+            CPS k F (tplus t1 t2) (fun res => res) 1 (depth F (tplus t1 t2))
+         =s CPS k F (tplus t1 t2) (fun res => res) 1 (1 + depth F t1)
+         =s CPS k F t1 (fun res : tm => tplus res t2) 1 (depth F t1)
+         =s tplus (CPS k F t1 (fun res => res) 1 (depth F t1)) t2 (TODO)
+       Finally,
+            subst F f' (CPS k F (tplus t1 t2) (fun res => res) 1 (depth F (tplus t1 t2)))
+         =s subst F f' (tplus (CPS k F t1 (fun res => res) 1 (depth F t1)) t2)
+         =s tplus (subst F f' (CPS k F t1 (fun res => res) 1 (depth F t1))) (subst F f' t2)
+         =s tplus (app k (subst F f t1)) t2
+         =s 
+         =s app k (tplus (subst F f t1) t2)
+         =s app k (subst F f (tplus t1 t2))
+         
+         
+         
+
+  The theorem to be informally proved:
+    subst F f' (CPS F M k 1 (depth F M)) =s k (subst F f M)
+
+  Proof:
+
+  By induction on M.
+
+  4. When M = tplus t1 t2.
+     The induction hypothesis:
+          subst F f' (CPS F t1 k 1 (depth F t1)) =s k (subst F f t1)
+          subst F f' (CPS F t2 k 1 (depth F t2)) =s k (subst F f t2)
+       ▲ If both t1 and t2 are not resursive,
+         We know that
+              CPS F t1 k 1 (depth F t1) = 
+       ▲ If t1 is recursive and t2 not recursive,
+       We know that,
+            
+*)
+
+Compute 1.
+
+Compute (CPS k F 
+<{ F a (F b c) }>
+ (fun res => res) 1 (depth F <{ F a (F b c) }>)).
+
+Compute (CPS k F 
+<{ F a (F b c) }>
+ (fun res => tplus res n2) 1 (depth F <{ F a (F b c) }>)).
+
+Compute (CPS k F 
+<{ F a (F b c) + n2 }>
+ (fun res => res) 1 (depth F <{ F a (F b c) + n2 }>)).
+
+Compute (tplus (CPS k F <{ F a (F b c) }> (fun res => res) 1 (depth F <{ F a (F b c) }>)) n2).
+
+Compute (CPS k F 
+<{ F a (F b c) }>
+ (fun res => res) 1 (depth F <{ F a (F b c) }>)).
+
+
+
+
+
